veric/Clight_new2.v
@@ -1,0 +1,403 @@
+Add LoadPath "..".
+Require Import veric.base.
+Require Import veric.Clight_lemmas.
+Require Import veric.sim. (*forward_simulations.
+Require Import veric.forward_simulations_proofs.*)
+
+Inductive cont': Type :=
+  | Kseq: statement -> cont'       (**r [Kseq s2 k] = after [s1] in [s1;s2] *)
+  | Kfor2: expr -> statement -> statement -> cont'       (**r [Kfor2 e2 e3 s k] = after [s] in [for'(e2;e3) s] *)
+  | Kfor3: expr -> statement -> statement  -> cont'       (**r [Kfor3 e2 e3 s k] = after [e3] in [for'(e2;e3) s] *)
+  | Kswitch: cont'       (**r catches [break] statements arising out of [switch] *)
+(*  | Kfun: fundef -> list val -> forall (l: option ident), cont' *)
+  | Kcall: forall (l: option ident),                  (**r where to store result *)
+           function ->                      (**r called (not calling!) function *)
+           env ->                           (**r local env of calling function *)
+           temp_env ->                      (**r temporary env of calling function *)
+           cont'.
+(*
+   | Kreturn: val -> cont'.
+*)
+
+Definition cont := list cont'.
+
+(** Pop continuation until a call or stop *)
+
+Fixpoint call_cont (k: cont) : cont :=
+  match k with
+  | Kseq s :: k => call_cont k
+  | Kfor2 e2 e3 s :: k => call_cont k
+  | Kfor3 e2 e3 s :: k => call_cont k
+  | Kswitch :: k => call_cont k
+  | _ => k
+  end.
+
+Fixpoint current_function (k: cont) : option function :=
+ match k with
+  | Kseq s :: k => current_function k
+  | Kfor2 e2 e3 s :: k => current_function k
+  | Kfor3 e2 e3 s :: k =>current_function k
+  | Kswitch :: k => current_function k
+  | Kcall _ f _ _ :: _ => Some f
+  | _ => None
+  end.
+
+Fixpoint continue_cont (k: cont) : cont :=
+  match k with
+  | Kseq s :: k' => continue_cont k'
+  | Kfor2 e2 e3 s :: k' => Kseq e3 :: Kfor3 e2 e3 s :: k'
+  | Kswitch :: k' => continue_cont k'
+  | _ => nil (* stuck *)
+  end.
+
+Fixpoint precontinue_cont (k: cont) : cont :=
+  match k with
+  | Kseq s :: k' => precontinue_cont k'
+  | Kfor2 _ _ _ :: _ => k
+  | Kswitch :: k' => precontinue_cont k'
+  | _ => nil (* stuck *)
+  end.
+
+Fixpoint break_cont (k: cont) : cont :=
+  match k with
+  | Kseq s :: k' => break_cont k'
+  | Kfor2 e2 e3 s :: k' => k'
+  | Kfor3 e2 e3 s :: _ => nil  (* stuck *)
+  | Kswitch :: k' => k'
+  | _ =>  nil (* stuck *)
+  end.
+
+Inductive corestate := 
+ | State: forall (ve: env) (te: temp_env) (k: cont), corestate
+ | ExtCall: forall (ef: external_function) (sig: signature) (args: list val) (lid: option ident) (ve: env) (te: temp_env) (k: cont),
+                corestate.
+
+Fixpoint strip_skip (k: cont) : cont :=
+ match k with Kseq Sskip :: k' => strip_skip k' | _ => k end.
+
+(*LENB: TYPE HAS CHANGED FROM option (external_function * signature * list val) 
+   to  option (external_function  * list val) 
+Definition cl_at_external (c: corestate) : option (external_function * signature * list val) :=
+  match c with
+  |  State _ _ k => None
+  | ExtCall ef sig args lid ve te k => Some (ef, sig, args)
+ end.*)
+Definition cl_at_external (c: corestate) : option (external_function * list val) :=
+  match c with
+  |  State _ _ k => None
+  | ExtCall ef sig args lid ve te k => Some (ef, args)
+ end.
+
+(*LENB: TYPE HAS CHANGED FROM  list val -> corestate -> option corestate
+   to  val -> corestate -> option corestate
+Definition cl_after_external (vret: val) (c: corestate) : option corestate :=
+  match vret, c with
+  | v, ExtCall ef sig args (Some id) ve te k => Some (State ve (PTree.set id v te) k)
+  | v, ExtCall ef sig args None ve te k => Some (State ve te k)
+  | _, _ => None
+  end.*)
+Definition cl_after_external (vret: val) (c: corestate) : option corestate :=
+  match vret, c with
+  | v, ExtCall ef sig args (Some id) ve te k => Some (State ve (PTree.set id v te) k)
+  | v, ExtCall ef sig args None ve te k => Some (State ve te k)
+  | _, _ => None
+  end.
+
+(** Find the statement and manufacture the continuation 
+  corresponding to a label *)
+
+Fixpoint find_label (lbl: label) (s: statement) (k: cont) 
+                    {struct s}: option cont :=
+  match s with
+  | Ssequence s1 s2 =>
+      match find_label lbl s1 (Kseq s2 :: k) with
+      | Some sk => Some sk
+      | None => find_label lbl s2 k
+      end
+  | Sifthenelse a s1 s2 =>
+      match find_label lbl s1 k with
+      | Some sk => Some sk
+      | None => find_label lbl s2 k
+      end
+  | Swhile a s1 =>
+      find_label lbl s1 (Kseq Scontinue :: Kfor2 a Sskip s1::  k)
+  | Sdowhile a s1 =>
+      find_label lbl s1 (Kseq Scontinue :: Kfor2 a Sskip s1 :: k)
+  | Sfor' a2 a3 s1 =>
+      match find_label lbl s1 (Kseq Scontinue :: Kfor2 a2 a3 s1 :: k) with
+      | Some sk => Some sk
+      | None => find_label lbl a3 (Kfor3 a2 a3 s1 :: k)
+      end
+  | Sswitch e sl =>
+      find_label_ls lbl sl (Kswitch :: k)
+  | Slabel lbl' s' =>
+      if ident_eq lbl lbl' then Some(Kseq s' :: k) else find_label lbl s' k
+  | _ => None
+  end
+
+with find_label_ls (lbl: label) (sl: labeled_statements) (k: cont) 
+                    {struct sl}: option cont :=
+  match sl with
+  | LSdefault s => find_label lbl s k
+  | LScase _ s sl' =>
+      match find_label lbl s (Kseq (seq_of_labeled_statement sl') :: k) with
+      | Some sk => Some sk
+      | None => find_label_ls lbl sl' k
+      end
+  end.
+
+
+(** Transition relation *)
+
+Inductive cl_step (ge: Clight.genv): forall (q: corestate) (m: mem) (q': corestate) (m': mem), Prop :=
+
+  | step_assign: forall ve te k m a1 a2 loc ofs v2 v t m',
+     type_is_volatile (typeof a1) = false ->
+      Clight_sem.eval_lvalue ge ve te m a1 loc ofs ->
+      Clight_sem.eval_expr ge ve te m a2 v2 ->
+      sem_cast v2 (typeof a2) (typeof a1) = Some v ->
+      Csem.assign_loc ge (typeof a1) m loc ofs v t m' ->
+      cl_step ge (State ve te (Kseq (Sassign a1 a2):: k)) m (State ve te k) m'
+
+  | step_set:   forall ve te k m id a v,
+      Clight_sem.eval_expr ge ve te m a v ->
+      cl_step ge (State ve te (Kseq (Sset id a) :: k)) m (State ve (PTree.set id v te) k) m
+
+  | step_call_internal:   forall ve te k m optid a al tyargs tyres vf vargs f m1 ve' le',
+      classify_fun (typeof a) = fun_case_f tyargs tyres ->
+      Clight_sem.eval_expr ge ve te m a vf ->
+      Clight_sem.eval_exprlist ge ve te m al tyargs vargs ->
+      Genv.find_funct ge vf = Some (Internal f) ->
+      type_of_function f = Tfunction tyargs tyres ->
+      list_norepet (var_names f.(fn_params) ++ var_names f.(fn_temps)) ->
+      Csem.alloc_variables empty_env m (f.(fn_vars)) ve' m1 ->
+      bind_parameter_temps f.(fn_params) vargs (create_undef_temps f.(fn_temps)) = Some 
+le' ->
+      cl_step ge (State ve te (Kseq (Scall optid a al) :: k)) m
+                   (State ve' le' (Kseq f.(fn_body) :: Kseq (Sreturn None) :: Kcall optid f ve te :: k)) m1
+
+  | step_call_external:   forall ve te k m optid a al tyargs tyres vf vargs ef,
+      classify_fun (typeof a) = fun_case_f tyargs tyres ->
+      Clight_sem.eval_expr ge ve te m a vf ->
+      Clight_sem.eval_exprlist ge ve te m al tyargs vargs ->
+      Genv.find_funct ge vf = Some (External ef tyargs tyres) ->
+      cl_step ge (State ve te (Kseq (Scall optid a al) :: k)) m (ExtCall ef (signature_of_type tyargs tyres) vargs optid ve te k) m
+
+  | step_seq: forall ve te k m s1 s2 st' m',
+          cl_step ge (State ve te (Kseq s1 :: Kseq s2 :: k)) m st' m' ->
+          cl_step ge (State ve te (Kseq (Ssequence s1 s2) :: k)) m st' m'
+
+  | step_skip: forall ve te k m st' m',
+          cl_step ge (State ve te k) m st' m' ->
+          cl_step ge (State ve te (Kseq Sskip :: k)) m st' m'
+
+  | step_continue: forall ve te k m st' m',
+           cl_step ge (State ve te (continue_cont k)) m st' m' ->
+           cl_step ge (State ve te (Kseq Scontinue :: k)) m st' m' 
+
+  | step_break: forall ve te k m st' m',
+                   cl_step ge (State ve te (break_cont k)) m st' m' ->
+                   cl_step ge (State ve te (Kseq Sbreak :: k)) m st' m'
+
+  | step_ifthenelse:  forall ve te k m a s1 s2 v1 b,
+      Clight_sem.eval_expr ge ve te m a v1 ->
+      bool_val v1 (typeof a) = Some b ->
+      cl_step ge (State ve te (Kseq (Sifthenelse a s1 s2) :: k)) m (State ve te  (Kseq (if b then s1 else s2) :: k)) m
+
+  | step_while: forall ve te k m a s st' m',
+      cl_step ge (State ve te (Kseq (Sfor' a Sskip s) :: k)) m st' m' ->
+      cl_step ge (State ve te (Kseq (Swhile a s) :: k)) m st' m'
+
+  | step_dowhile: forall ve te k m a s st' m',
+      cl_step ge (State ve te (Kseq s :: Kseq Scontinue :: Kfor2 a Sskip s :: k)) m st' m' ->
+      cl_step ge (State ve te (Kseq (Sdowhile a s) :: k)) m st' m'
+
+  | step_for: forall ve te k m a2 a3 s v2 b,
+      Clight_sem.eval_expr ge ve te m a2 v2 ->
+      bool_val v2 (typeof a2) = Some b ->
+      cl_step ge (State ve te (Kseq (Sfor' a2 a3 s) :: k)) m (State ve te (if b then Kseq s :: Kseq Scontinue :: Kfor2 a2 a3 s :: k else k)) m
+
+  | step_for3: forall ve te k m a2 a3 s v2 b,
+      Clight_sem.eval_expr ge ve te m a2 v2 ->
+      bool_val v2 (typeof a2) = Some b ->
+      cl_step ge (State ve te (Kfor3 a2 a3 s :: k)) m (State ve te (if b then Kseq s :: Kseq Scontinue :: Kfor2 a2 a3 s :: k else k)) m
+
+  | step_return: forall f ve te optexp optid k m v' m' ve' te' te'' k',
+      call_cont k = Kcall optid f ve' te' :: k' ->
+      Mem.free_list m (Csem.blocks_of_env ve) = Some m' ->
+      match optexp with None => True
+                                  | Some a => exists v, Clight_sem.eval_expr ge ve te m a v /\ sem_cast v (typeof a) f.(fn_return) = Some v' 
+                            end ->
+      match optid with None => f.(fn_return) = Tvoid /\ te''=te'
+                                | Some id => optexp <> None /\ te'' = PTree.set id v' te'
+      end ->
+      cl_step ge (State ve te (Kseq (Sreturn optexp) :: k)) m (State ve' te'' k') m'
+
+  | step_switch: forall ve te k m a sl n,
+      Clight_sem.eval_expr ge ve te m a (Vint n) ->
+      cl_step ge (State ve te (Kseq (Sswitch a sl) :: k)) m
+              (State ve te (Kseq (seq_of_labeled_statement (select_switch n sl)) :: Kswitch :: k)) m
+
+  | step_label: forall ve te k m lbl s st' m',
+       cl_step ge (State ve te (Kseq s :: k)) m st' m' ->
+       cl_step ge (State ve te (Kseq (Slabel lbl s) :: k)) m st' m'
+
+  | step_goto: forall f ve te k m lbl k'
+                     (* make sure to take a step here, so that every loop ticks the clock *) 
+      (CUR: current_function k = Some f),
+      find_label lbl f.(fn_body) (Kseq (Sreturn None) :: (call_cont k)) = Some k' ->
+      cl_step ge (State ve te (Kseq (Sgoto lbl) :: k)) m (State ve te k') m.
+
+Definition vret2v (vret: list val) : val :=
+  match vret with v::nil => v | _ => Vundef end.
+
+Definition exit_syscall_number : ident := 1%positive.
+
+(*LENB: TYPE HAS CHANGED FROM  genv -> corestate -> mem -> option val
+   to G -> C -> option int 
+Definition cl_safely_halted (ge: genv) (c: corestate) (m: mem) : option val := None.
+*)
+Definition cl_safely_halted (ge: genv) (c: corestate): option int := None.
+
+Definition empty_function : function := mkfunction Tvoid nil nil nil Sskip.
+
+Fixpoint temp_bindings (i: positive) (vl: list val) :=
+ match vl with
+ | nil => PTree.empty val
+ | v::vl' => PTree.set i v (temp_bindings (i+1)%positive vl')
+ end.
+
+Definition Tint32s := Tint I32 Signed noattr.
+Definition true_expr : Clight.expr := Clight.Econst_int Int.one Tint32s.
+
+Fixpoint typed_params (i: positive) (n: nat) : list (ident * type) :=
+ match n with
+ | O => nil
+ | S n' => (i, Tint32s) :: typed_params (i+1)%positive n'
+ end.
+
+Definition cl_initial_core (ge: genv) (v: val) (args: list val) : option corestate := 
+  let tl := typed_params 2%positive (length args)
+   in Some (State empty_env (temp_bindings 1%positive (v::args))
+                  (Kseq (Scall None 
+                                  (Etempvar 1%positive (Tfunction (type_of_params tl) Tvoid))
+                                  (map (fun x => Etempvar (fst x) (snd x)) tl)) :: 
+                     Kseq (Swhile true_expr Sskip) :: nil)).
+
+Lemma cl_corestep_not_at_external:
+  forall ge m q m' q', cl_step ge q m q' m' -> cl_at_external q = None.
+Proof.
+  intros.
+  destruct q; simpl; auto. inv H.
+Qed.
+
+(*LENB: TYPES HAVE CHANGED
+Lemma cl_corestep_not_halted :
+  forall ge m q m' q', cl_step ge q m q' m' -> cl_safely_halted ge q m = None.
+Proof.
+  intros.
+  simpl; auto.
+Qed.*)
+Lemma cl_corestep_not_halted :
+  forall ge m q m' q', cl_step ge q m q' m' -> cl_safely_halted ge q = None.
+Proof.
+  intros.
+  simpl; auto.
+Qed.
+
+Lemma cl_at_external_halted_excl :
+       forall ge q,cl_at_external q = None \/ cl_safely_halted ge q = None.
+ Proof. intros.  right. trivial. Qed.
+
+
+(*LENB: TYPE OF CoreSemantics HAS CHANGED
+Program Definition cl_core_sem : CoreSemantics (Genv.t fundef type) corestate mem external_function :=
+  @Build_CoreSemantics _ _ _ _
+    cl_initial_core
+    cl_at_external
+    cl_after_external
+    cl_safely_halted
+    cl_step
+    cl_corestep_not_at_external 
+    cl_corestep_not_halted _.
+*)
+
+Definition cl_init_mem (ge:genv)  (m:mem) d:  Prop:=
+   Genv.alloc_variables ge Mem.empty d = Some m.
+(*Defined initial memory, by adapting the definition of Genv.init_mem*)
+
+Definition cl_core_sem : CoreSemantics genv corestate mem  (list (ident * globvar type)) :=
+  @Build_CoreSemantics _ _ _ _ 
+    cl_init_mem
+    cl_initial_core
+    cl_at_external
+    cl_after_external
+    cl_safely_halted
+    cl_step
+    cl_corestep_not_at_external 
+    cl_corestep_not_halted
+    cl_at_external_halted_excl .
+
+(*
+Program Definition cl_core_sem : CoreSemantics (Genv.t fundef type) corestate mem.
+  eapply @Build_CoreSemantics with (corestep:=cl_step).
+       apply cl_init_mem.
+       apply  cl_initial_core.
+       apply cl_after_external.
+       apply cl_corestep_not_at_external.  
+       apply cl_corestep_not_halted.
+       intros. right; trivial.  Defined.
+*)
+
+Lemma cl_corestep_fun: forall ge m q m1 q1 m2 q2, 
+    cl_step ge q m q1 m1 -> 
+    cl_step ge q m q2 m2 -> 
+    (q1,m1)=(q2,m2).
+Proof.
+intros.
+rename H0 into STEP;
+revert q2 m2 STEP; induction H; intros; inv STEP; simpl; auto; repeat fun_tac; auto.
+inversion2 H H13. repeat fun_tac; auto.
+inversion2 H H7.
+destruct optexp. destruct H1 as [v [? ?]]. destruct H12 as [v2 [? ?]].
+repeat fun_tac.
+destruct optid. subst. auto. destruct H13,H2; subst; auto.
+destruct H2,H13; subst; auto.
+destruct optid; subst; auto. destruct H2; congruence.
+destruct H2,H13; subst; auto.
+inv H; auto.
+Qed.
+
+Lemma free_list_allowed_core_mod : forall m1 l m2,
+  Mem.free_list m1 l = Some m2 ->
+  allowed_core_modification m1 m2.
+Proof.
+  intros m1 l m2; revert m1; induction l; simpl; intros.
+  inv H;   eauto with allowed_mod.
+  destruct a; destruct p; invSome; eauto with allowed_mod.
+Qed.
+
+Hint Resolve free_list_allowed_core_mod : allowed_mod.
+
+Lemma cl_allowed_modifications : forall ge c m c' m',
+  cl_step ge c m c' m' -> allowed_core_modification m m'.
+Proof.
+  intros.
+  induction H; eauto with allowed_mod.
+  inv H3; eauto with allowed_mod. congruence.
+  admit.  (* need allowed_mod theorems about loadbytes and storebytes *)
+  apply allowed_core_modification_trans with m1.
+  clear - H5.
+  forget (fn_params f ++ fn_vars f) as l.
+  induction H5; eauto with allowed_mod.
+  forget (fn_params f) as l.
+  clear - H6; induction H6; eauto with allowed_mod.
+Qed.
+
+(*LENB: TYPE HAS CHANGED
+Definition cl_core_sem' : CompcertCoreSem (Genv.t fundef type) corestate external_function :=
+  Build_CompcertCoreSem _ _ _ cl_core_sem cl_corestep_fun cl_allowed_modifications.
+*)
+Definition cl_core_sem' : CompcertCoreSem (Genv.t fundef type) corestate (list (ident * globvar type)) :=
+  Build_CompcertCoreSem _ _ _ cl_core_sem  cl_corestep_fun cl_allowed_modifications.
+
