veric/Sim_starplus.v
@@ -1,0 +1,158 @@
+Add LoadPath "..".
+Require Import veric.base.
+Require Import compcert.Events.
+Require Import veric.sim. 
+
+(*Proofs that the individual cases of sim (sim_eq, sim_ext and sim_inj are closed under
+   star and plus. Then (presumably) lift this to compilercorrectness.*)
+
+(*SEVERAL HOLES IN THIS FILE!!!*)
+
+Section Sim_EQ_SIMU_DIAGRAMS.
+
+  Context {G1 C1 D1 G2 C2 D2:Type}
+          {Sem1 : CompcertCoreSem G1 C1 D1}
+          {Sem2 : CompcertCoreSem G2 C2 D2}
+
+          {ge1:G1}
+          {ge2:G2}
+          {entry_points : list (val * val * signature)}.
+
+  Variable core_data:Type.
+  Variable order: core_data -> core_data -> Prop.
+  Hypothesis order_wf: well_founded order.
+
+  Variable match_cores: core_data -> C1 -> C2 -> Prop.
+  Hypothesis match_initial_cores: 
+        forall v1 v2 sig, In (v1,v2,sig) entry_points ->
+        forall vals,  Forall2 (Val.has_type) vals (sig_args sig) ->
+       exists cd : core_data, exists c1 : C1, exists c2 : C2,
+                make_initial_core Sem1 ge1 v1 vals = Some c1 /\
+                make_initial_core Sem2 ge2 v2 vals = Some c2 /\ match_cores cd c1 c2.
+(*Smallstep/old version of this file had
+  Hypothesis match_initial_cores: 
+        forall v1 v2 sig, In (v1,v2,sig) entry_points ->
+        forall vals,  Forall2 (Val.has_type) vals (sig_args sig) ->
+        forall c1, make_initial_core Sem1 ge1 v1 vals = Some c1 ->
+                   exists c2, exists d, make_initial_core Sem2 ge2 v2 vals = Some c2 /\
+                                                   match_cores d c1 c2.
+*)
+
+  Hypothesis eq_safely_halted:
+      forall (cd : core_data) (c1 : C1) (c2 : C2) (v : int),
+      match_cores cd c1 c2 ->
+      safely_halted Sem1 ge1 c1 = Some v -> safely_halted Sem2 ge2 c2 = Some v.
+
+  Hypothesis eq_at_external: 
+         forall (d : core_data) (st1 : C1) (st2 : C2) (e : external_function) (args : list val),
+         match_cores d st1 st2 ->
+         at_external Sem1 st1 = Some (e, args) ->
+         at_external Sem2 st2 = Some (e, args) /\
+         Forall2 Val.has_type args (sig_args (ef_sig e)).
+
+  Hypothesis eq_after_external: forall (d : core_data) (st1 : C1) (st2 : C2) (ret : val)
+                                                                 (e : external_function) (args : list val),
+                      match_cores d st1 st2 ->
+                      at_external Sem1 st1 = Some (e, args) ->
+                      at_external Sem2 st2 = Some (e, args) ->
+                      Forall2 Val.has_type args (sig_args (ef_sig e)) ->
+                      Val.has_type ret (proj_sig_res (ef_sig e)) ->
+                      exists st1' : C1, exists st2' : C2, exists d' : core_data,
+                              after_external Sem1 ret st1 = Some st1' /\
+                              after_external Sem2 ret st2 = Some st2' /\ match_cores d' st1' st2'.
+
+Section SIMULATION_STAR_WF.
+  Hypothesis eq_simulation:
+     forall c1 m c1' m',  corestep Sem1 ge1 c1 m c1' m' ->
+     forall d c2, match_cores d c1 c2 ->
+      exists c2', exists d', match_cores d' c1' c2' /\
+                  (corestep_plus Sem2 ge2  c2 m c2' m' \/ (corestep_star Sem2 ge2 c2 m c2' m' /\ order d' d)).
+
+Lemma  eq_simulation_star_wf: Sim_eq.Forward_simulation_equals _ _ Sem1 Sem2 ge1 ge2 entry_points.
+Proof.
+  eapply Sim_eq.Build_Forward_simulation_equals with
+        (core_ord := order)
+        (match_core := match_cores). (*fun d c1 c2 => idx = s1 /\ match_cores c1 c2);*)
+   apply order_wf.
+   apply eq_simulation.
+   apply match_initial_cores.
+   apply eq_safely_halted.
+   apply eq_at_external.
+   apply eq_after_external.
+Qed.
+End SIMULATION_STAR_WF.
+
+Section SIMULATION_STAR.
+  Variable measure: C1 -> nat.
+  
+  Hypothesis eq_star_simulation:
+    forall c1 m c1' m', corestep Sem1 ge1 c1 m c1' m'  ->
+  forall d c2, match_cores d c1 c2 ->
+  (exists c2', exists d', corestep_plus Sem2 ge2 c2 m c2' m' /\ match_cores d' c1' c2' /\ order d' d)
+  \/ (measure c1' < measure c1 /\ m'=m /\ match_cores d c1' c2)%nat.
+
+  Definition star_data : Type := (core_data * C1)%type.
+  Definition star_ord:= lex_ord order (ltof _ measure).
+
+  Definition match_cores_star (cd:star_data) (c1:  C1) (c2: C2): Prop. 
+       destruct cd as [d c].
+       clear match_initial_cores eq_safely_halted eq_at_external eq_after_external eq_star_simulation.
+       apply ((match_cores d c1 c2) \/ (lt (measure c1) (measure c) /\ match_cores d c c2)).
+(*       apply (match_cores d c1 c2 \/ (lt (measure c1) (measure c) /\ match_cores d c c2)).*)
+  Defined. 
+
+Lemma  eq_simulation_star: Sim_eq.Forward_simulation_equals _ _ Sem1 Sem2 ge1 ge2 entry_points.
+Proof.
+  eapply Sim_eq.Build_Forward_simulation_equals with (core_ord:= star_ord)(match_core:=match_cores_star).
+       eapply wf_lex_ord. apply order_wf. apply (well_founded_ltof _ measure).
+      clear match_initial_cores eq_safely_halted eq_at_external eq_after_external.
+         unfold match_cores_star. intros. destruct d as [cd c].
+        specialize (eq_star_simulation _ _ _ _ H).  
+        destruct H0.  specialize (eq_star_simulation _ _ H0).
+                              destruct eq_star_simulation as [X | X]; clear eq_star_simulation.
+                                  (*case 1*) destruct X as [c2' [d' [CS [MC ORD]]]].
+                                                    exists c2'. exists (d', c). split. left; trivial. left; trivial.
+                                 (*case 2*) destruct X as [Measure [M MTCH]]. subst.
+                                                    exists st2. unfold star_ord.  exists (cd, st1). split. right; auto. 
+                                                             right. split. exists O. reflexivity.
+                                                                 apply lex_ord_right. unfold ltof. admit.  (*HERE's A HOLE!!*)
+            destruct H0. admit.
+    clear eq_star_simulation eq_after_external eq_at_external eq_safely_halted.
+        intros. specialize (match_initial_cores _ _ _ H _ H0).
+                   destruct match_initial_cores as [d [c1 [c2 [Ini1 [Ini2 MC]]]]].
+                   exists (d,c1). exists c1. exists c2. split; trivial. split; trivial.
+                   left; trivial.
+    clear eq_star_simulation eq_after_external eq_at_external match_initial_cores.
+        intros. destruct cd as [d c].
+                   destruct H. eapply (eq_safely_halted _ _ _ _ H H0).
+                   destruct H.  admit. (*HOLE*)
+    clear eq_after_external match_initial_cores eq_star_simulation eq_safely_halted.
+        intros. destruct d as [d c].
+                   destruct H. 
+                       eapply eq_at_external. apply H. apply H0.
+                   destruct H.  
+                       eapply eq_at_external. apply H1. admit. (*HOLE*)
+       (*afterexternal*)
+           admit.
+Qed.
+End SIMULATION_STAR.
+(** Simulation when one transition in the first program corresponds
+    to one or several transitions in the second program. *)
+
+Section SIMULATION_PLUS.
+
+Hypothesis eq_plus_simulation:
+  forall c1 m c1' m', corestep Sem1 ge1 c1 m c1' m'  ->
+  forall d c2, match_cores d c1 c2 ->
+  (exists c2', exists d', corestep_plus Sem2 ge2 c2 m c2' m' /\ match_cores d' c1' c2'  /\ order d' d).
+
+Lemma eq_simulation_plus: Sim_eq.Forward_simulation_equals _ _ Sem1 Sem2 ge1 ge2 entry_points.
+Proof.
+  apply eq_simulation_star with (measure := fun _ => O).
+  intros. left. clear eq_after_external eq_at_external  eq_safely_halted match_initial_cores.
+       apply (eq_plus_simulation _ _ _ _ H _ _ H0).
+Qed.
+
+End SIMULATION_PLUS.
+
+End Sim_EQ_SIMU_DIAGRAMS.
